Started Rely Guarantee Calculus for infinite trace model

Models/Evaluation.thy
@@ -1,21 +1,6 @@
 theory Evaluation
-  imports Language
+  imports Language Topped
 begin
-
-definition pow_inv :: "'a set \<Rightarrow> 'a lan" ("\<iota>") where
-  "pow_inv X \<equiv> {xs. lset xs \<subseteq> X}"
-
-definition symbols :: "'a lan \<Rightarrow> 'a set" ("\<rho>") where
-  "symbols X \<equiv> \<Union>xs\<in>X. lset xs"
-
-lemma galois_connection: "\<rho> X \<subseteq> Y \<longleftrightarrow> X \<subseteq> \<iota> Y"
-  by (auto simp add: pow_inv_def symbols_def)
-
-lemma \<rho>_iso: "X \<subseteq> Y \<Longrightarrow> \<rho> X \<subseteq> \<rho> Y"
-  by (metis Int_absorb1 galois_connection le_infI1 order_refl)
-
-lemma \<iota>_iso: "X \<subseteq> Y \<Longrightarrow> \<iota> X \<subseteq> \<iota> Y"
-  by (metis galois_connection order_refl order_trans)
 
 lemma (in complete_lattice) Inf_singleton: "Inf {x} = x"
   by (smt Inf_empty Inf_insert inf_top_right)
@@ -275,118 +260,6 @@ lemma steps_singleton: "\<sigma> \<in> P \<Longrightarrow> steps xs {\<sigma>} =
   apply simp
   by (metis empty_subsetI efw_iso insert_absorb insert_mono subset_empty)
 
-datatype 'a top = Top | NotTop 'a
-
-abbreviation bind :: "('a \<Rightarrow> 'b top) \<Rightarrow> 'a top \<Rightarrow> 'b top" (infixr "\<hookleftarrow>" 56)  where
-  "bind f x \<equiv> case x of Top \<Rightarrow> Top | NotTop x \<Rightarrow> f x"
-
-lemma top_left_id: "f \<hookleftarrow> NotTop x = f x"
-  by auto
-
-lemma top_right_id: "NotTop \<hookleftarrow> x = x"
-  by (cases x) auto
-
-lemma top_assoc: "g \<hookleftarrow> f \<hookleftarrow> x = (\<lambda>x. g \<hookleftarrow> (f x)) \<hookleftarrow> x"
-  by (cases x) auto
-
-instantiation top :: (ord) ord
-begin
-  definition less_eq_top :: "'a top \<Rightarrow> 'a top \<Rightarrow> bool" where
-    "x \<le> y \<equiv> case y of Top \<Rightarrow> True | NotTop y \<Rightarrow> case x of Top \<Rightarrow> False | NotTop x \<Rightarrow> x \<le> y"
-
-  definition less_top :: "'a top \<Rightarrow> 'a top \<Rightarrow> bool" where
-    "less_top x y \<equiv> x \<le> y \<and> \<not> (y \<le> x)"
-
-  instance by default
-end
-
-instance top :: (order) order
-proof
-  fix x y z :: "'a top"
-  show "(x < y) = (x \<le> y \<and> \<not> y \<le> x)"
-    by (simp add: less_top_def)
-  show "x \<le> x"
-    by (cases x) (auto simp add: less_eq_top_def)
-  show "x \<le> y \<Longrightarrow> y \<le> z \<Longrightarrow> x \<le> z"
-    apply (cases x)
-    apply (cases y, cases z, (force simp add: less_eq_top_def)+)
-    apply (cases y, cases z, (force simp add: less_eq_top_def)+)
-    by (cases z, (force simp add: less_eq_top_def)+)
-  show "x \<le> y \<Longrightarrow> y \<le> x \<Longrightarrow> x = y"
-    by (cases x) (cases y, (force simp add: less_eq_top_def)+)+
-qed
-
-lemma NotTop_mono [intro!]: "x \<le> y \<Longrightarrow> NotTop x \<le> NotTop y"
-  by (auto simp add: less_eq_top_def)
-
-instantiation top :: (lattice) lattice
-begin
-  definition sup_top :: "'a top \<Rightarrow> 'a top \<Rightarrow> 'a top" where
-    "sup_top x y \<equiv> case x of Top \<Rightarrow> Top | NotTop x \<Rightarrow> (case y of Top \<Rightarrow> Top | NotTop y \<Rightarrow> NotTop (sup x y))"
-
-  definition inf_top :: "'a top \<Rightarrow> 'a top \<Rightarrow> 'a top" where
-    "inf_top x y \<equiv> case x of Top \<Rightarrow> y | NotTop x \<Rightarrow> (case y of Top \<Rightarrow> NotTop x | NotTop y \<Rightarrow> NotTop (inf x y))"  
-
-  instance
-  proof
-    fix x y z :: "'a top"
-    show "inf x y \<le> x"
-      sorry
-    show "inf x y \<le> y"
-      sorry
-    show "x \<le> y \<Longrightarrow> x \<le> z \<Longrightarrow> x \<le> inf y z"
-      sorry
-    show "x \<le> sup x y"
-      sorry
-    show "y \<le> sup x y"
-      sorry
-    show "y \<le> x \<Longrightarrow> z \<le> x \<Longrightarrow> sup y z \<le> x"
-      sorry
-  qed
-end
-
-instantiation top :: (complete_lattice) complete_lattice
-begin
-  definition Inf_top :: "'a top set \<Rightarrow> 'a top" where "Inf_top \<equiv> undefined"
-
-  definition Sup_top :: "'a top set \<Rightarrow> 'a top" where "Sup_top X \<equiv> if Top \<in> X then Top else NotTop (Sup {x. NotTop x \<in> X})"
-
-  definition top_top :: "'a top" where "top_top = Top"
-
-  definition bot_top :: "'a top" where "bot_top = NotTop bot"
-
-  instance
-  proof
-    fix a :: "'a top"
-    show "a \<le> top"
-      by (cases a) (auto simp add: top_top_def less_eq_top_def)
-    show "bot \<le> a"
-      by (cases a) (auto simp add: bot_top_def less_eq_top_def)
-  next
-    fix x :: "'a top" and A :: "'a top set"
-    assume xA: "x \<in> A"
-    show "Inf A \<le> x"
-      sorry
-    show "x \<le> Sup A"
-      by (insert xA, cases x, auto intro: Sup_upper simp add: Sup_top_def less_eq_top_def) 
-  next
-    fix z :: "'a top" and A :: "'a top set"
-    assume "\<And>x. x \<in> A \<Longrightarrow> z \<le> x"
-    thus "z \<le> Inf A"
-      sorry
-  next
-    fix z :: "'a top" and A :: "'a top set"
-    assume "\<And>x. x \<in> A \<Longrightarrow> x \<le> z"
-    thus "Sup A \<le> z"
-      apply (cases z)
-      apply (auto intro!: Sup_least simp add: Sup_top_def less_eq_top_def)
-      apply (metis top.simps(4))
-      by (metis (full_types) top.simps(5))
-  qed
-end
-
-lemma [simp]: "f \<hookleftarrow> top = top" by (simp add: top_top_def)
-
 definition eval_word :: "'a rel llist \<Rightarrow> 'a set \<Rightarrow> 'a set top" where
   "eval_word xs H \<equiv> case steps xs H of \<infinity> \<Rightarrow> top | enat n \<Rightarrow> NotTop (eval_finite_word (list_of (ltake (enat n) xs)) H)"
 
@@ -429,12 +302,6 @@ lemma all_terminating_word1: "\<nabla>X = bot \<longleftrightarrow> \<not> (\<ex
 
 lemmas all_terminating_word = all_terminating_word1[simplified]
 
-lemma [simp]: "inf (NotTop x) (NotTop y) = NotTop (x \<inter> y)"
-  by (simp add: inf_top_def)
-
-lemma [simp]: "NotTop x = bot \<longleftrightarrow> x = {}"
-  by (simp add: bot_top_def)
-
 lemma non_terminating_word_var: "inf (\<nabla>X) (NotTop Y) \<noteq> bot \<longleftrightarrow> (\<exists>xs\<in>X. \<exists>\<sigma>\<in>Y. steps xs {\<sigma>} = \<infinity>)" 
   by (auto simp add: nabla_def llist_nabla_def)
 
@@ -473,8 +340,6 @@ proof -
     by (simp_all add: nabla_def module_def)
 qed
 
-lemmas Top_top = top_top_def[symmetric]
-
 lemma [simp]: "Top \<le> NotTop x \<longleftrightarrow> False"
   by (simp add: less_eq_top_def)
 
@@ -487,7 +352,7 @@ lemma mod_isol: "p \<le> q \<Longrightarrow> x \<Colon> p \<le> x \<Colon> q"
   apply (cases q)
   apply (auto simp add: module_def)
   apply (rule Sup_mono)
-  apply (auto simp add: Top_top)
+  apply (auto simp add: top_top_def[symmetric])
   apply (cases p)
   apply auto
   apply (rule Sup_mono)
@@ -507,8 +372,6 @@ lemma mod_distl: "(x \<Colon> p) \<squnion> (x \<Colon> q) \<le> x \<Colon> (p \
 
 lemma mod_distr: "(x \<union> y) \<Colon> p = (x \<Colon> p) \<squnion> (y \<Colon> p)"
   by (auto intro: arg_cong[where f = Sup] simp add: module_def Sup_union_distrib[symmetric])
-
-declare Top_top[simp]
 
 lemma [simp]: "x \<noteq> {} \<Longrightarrow> x \<Colon> top = top"
   by (auto intro!: Sup_top_eq_top simp add: module_def)
@@ -739,7 +602,7 @@ lemma infinite_eval_cases: "X \<cdot> {} \<Colon> h = top \<or> X \<cdot> {} \<C
   apply (cases "X \<cdot> {} = {}")
   apply simp
   apply (cases h)
-  apply simp
+  apply (simp add: Top_top)
   apply (simp add: bot_top_def)
   apply (rule INF_part_mod1)
   by auto
@@ -749,9 +612,9 @@ lemma [simp]: "x \<triangleright> top = top"
 
 lemma mod2_infinite_eval_cases: "X \<cdot> {} \<triangleright> h = top \<or> X \<cdot> {} \<triangleright> h = bot"
   apply (cases h)
-  apply simp
+  apply (simp add: Top_top)
   apply (cases "X \<cdot> {} = {}")
-  apply simp
+  apply (simp add: Top_top)
   apply (erule ssubst)
   apply (subst bot_top_def)
   apply (rule INF_part_mod2)
@@ -767,33 +630,14 @@ lemma mod2_infinite: "x \<cdot> {} \<triangleright> h \<le> y \<triangleright> x
 lemma "y \<noteq> {} \<Longrightarrow> (x \<cdot> {} \<Colon> h) = y \<Colon> (x \<cdot> {} \<Colon> h)"
   by (rule disjE[OF infinite_eval_cases[of x h]]) simp_all
 
-lemma eval_word_finite: "lfinite w \<Longrightarrow> eval_word w h = NotTop (eval_finite_word (list_of w) h)"
-  apply (simp add: eval_word_def)
-  apply (rule sym)
-  apply simp
-  apply (simp add: steps_def)
-  apply (cases "llength w \<le> Inf {enat n |n. eval_finite_word (list_of (ltake (enat n) w)) h = {}}")
-  apply (subst min_max.inf_absorb1)
-  apply assumption
-  apply (metis lfinite_llength_enat ltake_llength)
-  apply (drule linearD)
-  apply (subst min_max.inf_absorb2)
-  apply simp
-  apply (simp add: lfinite_conv_llength_enat)
-  apply (erule exE)
-  sorry
-
 lemma helper: "(\<And>x. P x \<Longrightarrow> f x = g x) \<Longrightarrow> (\<And>x. Q x \<Longrightarrow> P x) \<Longrightarrow> {f x |x. Q x} = {g x |x. Q x}"
   by auto metis
 
 lemma NotTop_continuous: "NotTop (\<Union>X) = Sup (NotTop ` X)"
-  by (auto simp add: Sup_top_def) (metis top.distinct(1) top_top_def)
+  by (auto simp add: Sup_top_def Top_top) (metis top.distinct(1) top_top_def)
 
 lemma [simp]: "f ` {g x |x. P x} = {f (g x) |x. P x}"
   by (auto simp add: image_def)
-
-lemma "x \<inter> FIN \<Colon> (NotTop h) = NotTop (\<Union>{eval_finite_word (list_of w) h |w. w \<in> x \<and> w \<in> FIN})"
-  by (auto intro: arg_cong[where f = Sup] eval_word_finite eval_word_finite[symmetric] simp: module_def FIN_def NotTop_continuous)
 
 lemma (in complete_lattice) Sup_eq_bot: "X = {} \<Longrightarrow> Sup X = bot"
   by simp
@@ -804,8 +648,8 @@ lemma [simp]: "inf (NotTop p) (NotTop q) = NotTop (p \<inter> q)"
 lemma [simp]: "\<Union>X \<inter> Y = {} \<longleftrightarrow> (\<forall>X'\<in>X. X' \<inter> Y = {})"
   by auto
 
-lemma [simp]: "top = bot \<longleftrightarrow> False"
-  sorry
+lemma [simp]: "(top :: 'a::complete_lattice top) = bot \<longleftrightarrow> False"
+  by (simp add: top_top_def bot_top_def)
 
 lemma [intro!]: "\<exists>m'. m = enat m' \<and> f m' = Y \<Longrightarrow> (case m of enat n \<Rightarrow> NotTop (f n) | \<infinity> \<Rightarrow> top) = NotTop Y"
   apply (cases m)
@@ -901,11 +745,11 @@ lemma eval_word_continuous: "Sup (eval_word w ` X) \<le> eval_word w (\<Union>X)
   by (smt Sup_le_iff Sup_upper eval_word_iso image_iff)
 
 lemma Sup_no_top: "top \<notin> X \<Longrightarrow> Sup X = NotTop (\<Union>{x. \<exists>y. y = NotTop x \<and> y \<in> X})"
-  by (simp add: Sup_top_def)
+  by (simp add: Sup_top_def Top_top)
 
 lemma Sup_bind: "Sup {f \<hookleftarrow> x |x. x \<in> X} = Sup ((f ` {x. \<exists>y. y = NotTop x \<and> y \<in> X}) \<union> (if top \<in> X then {top} else {}))"
   apply auto
-  apply (simp add: Sup_top_def)
+  apply (simp add: Sup_top_def Top_top)
   apply (rule_tac x = top in exI)
   apply simp
   apply (simp add: image_def)
@@ -928,7 +772,7 @@ proof -
   also have "... \<le> eval_word w (\<Union>{x. \<exists>y. y = NotTop x \<and> y \<in> X}) \<squnion> Sup (if top \<in> X then {top} else {})"
     by (rule sup_mono[OF eval_word_continuous order_refl])
   also have "... \<le> eval_word w \<hookleftarrow> Sup X"
-    by (auto simp add: Sup_top_def) (metis bot_least bot_top_def)
+    by (auto simp add: Sup_top_def Top_top) (metis bot_least bot_top_def)
   finally show ?thesis .
 qed
 
@@ -980,14 +824,9 @@ lemma infinite_inter [simp]: "x \<inter> - FIN = x \<cdot> {}"
 
 lemma "x \<noteq> {} \<Longrightarrow> x \<Colon> p \<le> q \<Longrightarrow> x \<triangleright> p \<le> q"
   apply (cases p)
-  apply (simp)
+  apply (simp add: Top_top)
   apply (simp only: top_top_def module2.simps)
   by (simp add: module_def)
-
-find_theorems "op \<Colon>"
-
-lemma [simp]: "x \<triangleright> top = top"
-  by (metis module2.simps(1) top_top_def)
 
 lemma mod2_distr: "x \<union> y \<triangleright> p = (x \<triangleright> p) \<squnion> (y \<triangleright> p)"
   by (cases p) simp_all
@@ -1000,6 +839,25 @@ lemma mod2_distl: "(x \<triangleright> p) \<squnion> (x \<triangleright> q) \<le
   apply (auto intro!: Sup_mono)
   apply (metis inf_sup_ord(3))
   by (metis inf_sup_ord(4))
+
+lemma mod2_isol: "x \<le> y \<Longrightarrow> x \<triangleright> p \<le> y \<triangleright> p"
+  by (cases p) (auto intro: Sup_mono)
+
+thm mod_isor
+
+lemma mod2_isor: "p \<le> q \<Longrightarrow> x \<triangleright> p \<le> x \<triangleright> q"
+  apply (cases q)
+  apply simp
+  apply (cases p)
+  apply simp
+  apply simp
+  apply (rule Sup_mono)
+  apply auto
+  apply (rule_tac x = "eval_word w a" in exI)
+  apply (intro conjI)
+  apply (rule_tac x = w in exI)
+  apply simp
+  by (metis eval_word_iso)
 
 lemma mod_le_mod2: "x \<Colon> p \<le> x \<triangleright> p"
   by (cases p) (simp_all add: module_def)
@@ -1037,45 +895,5 @@ proof -
   thus ?thesis
     by (cases p) simp_all
 qed
-    
-
-
-lemma mod_mult:
-  assumes "y \<noteq> {}"
-  shows "x \<cdot> y \<Colon> p \<le> y \<Colon> x \<Colon> p"
-proof -
-  have "x \<cdot> y \<Colon> p = Sup {eval_word w \<hookleftarrow> p |w . w \<in> x \<cdot> y}"
-    by (simp add: module_def)
-  also have "... = Sup {eval_word w \<hookleftarrow> p |w. w \<in> x \<and> \<not> lfinite w} \<squnion> Sup {eval_word w \<hookleftarrow> p |w. \<exists>xs ys. w = xs \<frown> ys \<and> xs \<in> x \<and> lfinite xs \<and> ys \<in> y}"
-    by (simp add: l_prod_def)
-  also have "... = Sup {eval_word w \<hookleftarrow> p |w. w \<in> x \<and> \<not> lfinite w} \<squnion> Sup {eval_word (xs \<frown> ys) \<hookleftarrow> p |xs ys. xs \<in> x \<and> lfinite xs \<and> ys \<in> y}"
-    by (rule arg_cong, blast)
-  also have "... = Sup {eval_word w \<hookleftarrow> p |w. w \<in> x \<and> \<not> lfinite w} \<squnion> Sup {eval_word ys \<hookleftarrow> eval_word xs \<hookleftarrow> p |xs ys. xs \<in> x \<and> lfinite xs \<and> ys \<in> y}"
-    by (rule arg_cong, force simp add: eval_word_lappend)
-  also have "... = Sup {eval_word w \<hookleftarrow> p |w. w \<in> x \<and> \<not> lfinite w} \<squnion> Sup {Sup {eval_word ys \<hookleftarrow> eval_word xs \<hookleftarrow> p |xs. xs \<in> x \<and> lfinite xs} |ys. ys \<in> y}"
-    by simp
-  also have "... = Sup {eval_word w \<hookleftarrow> p |w. w \<in> x \<and> \<not> lfinite w} \<squnion> Sup {Sup {eval_word ys \<hookleftarrow> eval_word xs \<hookleftarrow> p |xs. xs \<in> (x \<inter> FIN)} |ys. ys \<in> y}"
-    by (simp add: FIN_def)
-  also have "... = Sup {eval_word w \<hookleftarrow> p |w. w \<in> x \<and> \<not> lfinite w} \<squnion> Sup {Sup {eval_word ys \<hookleftarrow> q |q. q \<in> {eval_word xs \<hookleftarrow> p |xs. xs \<in> x \<inter> FIN}} |ys. ys \<in> y}"
-    by (rule arg_cong, rule comp_f_eq, rule arg_cong, auto)
-  also have "... \<le> Sup {eval_word w \<hookleftarrow> p |w. w \<in> x \<and> \<not> lfinite w} \<squnion> Sup {eval_word ys \<hookleftarrow> Sup {eval_word xs \<hookleftarrow> p |xs. xs \<in> (x \<inter> FIN)} |ys. ys \<in> y}"
-    by (rule sup_mono[OF order_refl], rule Sup_comp_f_mono, rule eval_word_bind_continuous)
-  also have "... = Sup {eval_word w \<hookleftarrow> p |w. w \<in> x \<and> \<not> lfinite w} \<squnion> (y \<Colon> (x \<inter> FIN) \<Colon> p)"
-    by (simp add: module_def)
-  also have "... = Sup {eval_word w \<hookleftarrow> p |w. w \<in> x \<inter> - FIN} \<squnion> (y \<Colon> (x \<inter> FIN) \<Colon> p)"
-    by (simp add: FIN_def)
-  also have "... = (x \<inter> - FIN \<Colon> p) \<squnion> (y \<Colon> x \<inter> FIN \<Colon> p)"
-    by (simp add: module_def)
-  also have "... = (y \<Colon> x \<inter> - FIN \<Colon> p) \<squnion> (y \<Colon> x \<inter> FIN \<Colon> p)"
-    by simp (metis (hide_lams, no_types) assms infinite_eval_cases le_iff_sup mod_isol mod_top sup_bot_left sup_commute sup_top_left)
-  also have "... \<le> y \<Colon> x \<Colon> p"
-    by (metis Int_lower1 le_sup_iff mod_isol mod_isor)
-  finally show ?thesis .
-qed
-
-lemma "x \<cdot> y \<triangleright> p \<le> y \<triangleright> x \<triangleright> p"
-  sledgehammer
-
-end
 
 end
