Models/RelyGuarantee.thy
@@ -1,0 +1,67 @@
+theory RelyGuarantee
+  imports PowerInvariant Evaluation
+begin
+
+no_notation
+  Transitive_Closure.trancl ("(_\<^sup>+)" [1000] 999)
+
+definition trancl :: "'a lan \<Rightarrow> 'a lan" ("_\<^sup>+" [101] 100) where
+  "x\<^sup>+ \<equiv> x\<cdot>x\<^sup>\<star>"
+
+definition I :: "'a lan set" where
+  "I \<equiv> {x. \<exists>y. x = \<iota> y}"
+
+definition quintuple :: "'a rel lan \<Rightarrow> 'a rel lan \<Rightarrow> 'a set top \<Rightarrow> 'a rel lan \<Rightarrow> 'a set top \<Rightarrow> bool" ("_, _ \<turnstile> \<lbrace>_\<rbrace> _ \<lbrace>_\<rbrace>") where
+  "r, g \<turnstile> \<lbrace>p\<rbrace> c \<lbrace>q\<rbrace> \<longleftrightarrow> r \<parallel> c \<triangleright> p \<le> q \<and> c \<le> g \<and> r \<in> I \<and> g \<in> I"
+
+lemma inv_dist:
+  assumes "r \<in> I" shows "r\<parallel>(x\<cdot>y) \<le> (r\<parallel>x)\<cdot>(r\<parallel>y)"
+proof -
+  obtain r' where [simp]: "r = \<iota> r'"
+    using assms by (auto simp: I_def)
+  thus ?thesis by simp (rule pow_inv1)
+qed
+
+lemma inv_mult_par: "r \<in> I \<Longrightarrow> s \<in> I \<Longrightarrow> r \<cdot> s \<le> r \<parallel> s"
+  apply (simp add: I_def)
+  apply (erule exE)+
+  apply simp
+  by (metis fin_l_prod_le_shuffle pow_inv_finite)
+
+lemma inv_par_closed: "r \<in> I \<Longrightarrow> s \<in> I \<Longrightarrow> r \<parallel> s \<in> I"
+  sorry
+
+lemma sequential:
+  assumes "r, g1 \<turnstile> \<lbrace>p\<rbrace> c1 \<lbrace>q\<rbrace>" and "r, g2 \<turnstile> \<lbrace>q\<rbrace> c2 \<lbrace>s\<rbrace>"
+  shows "r, (g1 \<parallel> g2) \<turnstile> \<lbrace>p\<rbrace> c1 \<cdot> c2 \<lbrace>s\<rbrace>"
+proof -
+  have r_inv: "r \<in> I"
+    by (metis assms(1) quintuple_def)
+
+  {
+    have "r \<parallel> (c1 \<cdot> c2) \<triangleright> p \<le> (r \<parallel> c1) \<cdot> (r \<parallel> c2) \<triangleright> p"
+      by (metis inv_dist mod2_isol r_inv)
+    also have "... \<le> r \<parallel> c2 \<triangleright> r \<parallel> c1 \<triangleright> p"
+      by (metis mod2_mult)
+    also have "... \<le> r \<parallel> c2 \<triangleright> q"
+      by (metis assms(1) mod2_isor quintuple_def)
+    also have "... \<le> s"
+      by (metis assms(2) quintuple_def)
+    finally have "r \<parallel> (c1 \<cdot> c2) \<triangleright> p \<le> s" .
+  }
+  moreover
+  {
+    have "c1 \<cdot> c2 \<le> g1 \<cdot> g2"
+      by (metis assms(1) assms(2) quintuple_def seq.mult_isol_var)
+    also have "... \<le> g1 \<parallel> g2"
+      by (metis assms(1) assms(2) inv_mult_par quintuple_def)
+    finally have "c1 \<cdot> c2 \<le> g1 \<parallel> g2" .
+  }
+  ultimately show ?thesis
+    by (metis assms(1) assms(2) inv_par_closed quintuple_def)
+qed
+
+lemma parallel
+  
+
+end
