Models/Topped.thy
@@ -1,0 +1,148 @@
+theory Topped
+  imports Main
+begin
+
+datatype 'a top = Top | NotTop 'a
+
+abbreviation bind :: "('a \<Rightarrow> 'b top) \<Rightarrow> 'a top \<Rightarrow> 'b top" (infixr "\<hookleftarrow>" 56)  where
+  "bind f x \<equiv> case x of Top \<Rightarrow> Top | NotTop x \<Rightarrow> f x"
+
+lemma top_left_id: "f \<hookleftarrow> NotTop x = f x"
+  by simp
+
+lemma top_right_id: "NotTop \<hookleftarrow> x = x"
+  by (cases x) auto
+
+lemma top_assoc: "g \<hookleftarrow> f \<hookleftarrow> x = (\<lambda>x. g \<hookleftarrow> (f x)) \<hookleftarrow> x"
+  by (cases x) auto
+
+instantiation top :: (ord) ord
+begin
+  definition less_eq_top :: "'a top \<Rightarrow> 'a top \<Rightarrow> bool" where
+    "x \<le> y \<equiv> case y of Top \<Rightarrow> True | NotTop y \<Rightarrow> case x of Top \<Rightarrow> False | NotTop x \<Rightarrow> x \<le> y"
+
+  definition less_top :: "'a top \<Rightarrow> 'a top \<Rightarrow> bool" where
+    "less_top x y \<equiv> x \<le> y \<and> \<not> (y \<le> x)"
+
+  instance by default
+end
+
+instance top :: (order) order
+proof
+  fix x y z :: "'a top"
+  show "(x < y) = (x \<le> y \<and> \<not> y \<le> x)"
+    by (simp add: less_top_def)
+  show "x \<le> x"
+    by (cases x) (auto simp add: less_eq_top_def)
+  show "x \<le> y \<Longrightarrow> y \<le> z \<Longrightarrow> x \<le> z"
+    apply (cases x)
+    apply (cases y, cases z, (force simp add: less_eq_top_def)+)
+    apply (cases y, cases z, (force simp add: less_eq_top_def)+)
+    by (cases z, (force simp add: less_eq_top_def)+)
+  show "x \<le> y \<Longrightarrow> y \<le> x \<Longrightarrow> x = y"
+    by (cases x) (cases y, (force simp add: less_eq_top_def)+)+
+qed
+
+lemma [simp, intro!]: "x \<le> Top"
+  by (simp add: less_eq_top_def)
+
+lemma [simp]: "Top \<le> x \<longleftrightarrow> x = Top"
+  by (cases x) (simp_all add: less_eq_top_def)
+
+lemma NotTop_mono: "x \<le> y \<Longrightarrow> NotTop x \<le> NotTop y"
+  by (auto simp add: less_eq_top_def)
+
+lemma [simp]: "NotTop x \<le> NotTop y \<longleftrightarrow> x \<le> y"
+  by (auto simp add: less_eq_top_def)  
+
+instantiation top :: (lattice) lattice
+begin
+  definition sup_top :: "'a top \<Rightarrow> 'a top \<Rightarrow> 'a top" where
+    "sup_top x y \<equiv> case x of Top \<Rightarrow> Top | NotTop x \<Rightarrow> (case y of Top \<Rightarrow> Top | NotTop y \<Rightarrow> NotTop (sup x y))"
+
+  definition inf_top :: "'a top \<Rightarrow> 'a top \<Rightarrow> 'a top" where
+    "inf_top x y \<equiv> case x of Top \<Rightarrow> y | NotTop x \<Rightarrow> (case y of Top \<Rightarrow> NotTop x | NotTop y \<Rightarrow> NotTop (inf x y))"  
+
+  lemma [simp]: "inf Top y = y"
+    by (simp add: inf_top_def)
+
+  lemma [simp]: "inf x Top = x"
+    by (cases x) (simp_all add: inf_top_def)
+
+  lemma [simp]: "inf (NotTop x) (NotTop y) = NotTop (inf x y)"
+    by (simp add: inf_top_def)
+
+  lemma [simp]: "sup Top y = Top"
+    by (simp add: sup_top_def)
+
+  lemma [simp]: "sup x Top = Top"
+    by (cases x) (simp_all add: sup_top_def)
+
+  lemma [simp]: "sup (NotTop x) (NotTop y) = NotTop (sup x y)"
+    by (simp add: sup_top_def)
+
+  instance
+  proof
+    fix x y z :: "'a top"
+    show "inf x y \<le> x"
+      by (simp add: inf_top_def, cases x, simp, cases y, auto)
+    show "inf x y \<le> y"
+      by (simp add: inf_top_def, cases x, simp, cases y, auto)
+    show "x \<le> y \<Longrightarrow> x \<le> z \<Longrightarrow> x \<le> inf y z"
+      by (cases x, simp, cases y, simp, cases z, auto)
+    show "x \<le> sup x y"
+      by (cases x, simp, cases y, auto)
+    show "y \<le> sup x y"
+      by (cases x, simp, cases y, auto)
+    show "y \<le> x \<Longrightarrow> z \<le> x \<Longrightarrow> sup y z \<le> x"
+      by (cases x, simp, cases y, simp, cases z, auto)
+  qed
+end
+
+find_theorems "Inf" "{}"
+
+instantiation top :: (complete_lattice) complete_lattice
+begin
+  definition Inf_top :: "'a top set \<Rightarrow> 'a top" where "Inf_top X \<equiv> if X \<subseteq> {Top} then Top else NotTop (Inf {x. NotTop x \<in> X})"
+
+  definition Sup_top :: "'a top set \<Rightarrow> 'a top" where "Sup_top X \<equiv> if Top \<in> X then Top else NotTop (Sup {x. NotTop x \<in> X})"
+
+  definition top_top :: "'a top" where "top_top = Top"
+
+  definition bot_top :: "'a top" where "bot_top = NotTop bot"
+
+  instance
+  proof
+    fix a :: "'a top"
+    show "a \<le> top"
+      by (cases a) (auto simp add: top_top_def less_eq_top_def)
+    show "bot \<le> a"
+      by (cases a) (auto simp add: bot_top_def less_eq_top_def)
+  next
+    fix x :: "'a top" and A :: "'a top set"
+    assume xA: "x \<in> A"
+    show "Inf A \<le> x" using xA
+      by (cases x) (auto intro: Inf_lower simp: Inf_top_def)
+    show "x \<le> Sup A" using xA
+      by (cases x) (auto intro: Sup_upper simp add: Sup_top_def less_eq_top_def) 
+  next
+    fix z :: "'a top" and A :: "'a top set"
+    assume "\<And>x. x \<in> A \<Longrightarrow> z \<le> x"
+    thus "z \<le> Inf A"
+      apply (cases z)
+      apply (auto simp add: Inf_top_def)
+      by (metis (lifting, no_types) le_Inf_iff less_eq_top_def mem_Collect_eq top.simps(5))
+  next
+    fix z :: "'a top" and A :: "'a top set"
+    assume "\<And>x. x \<in> A \<Longrightarrow> x \<le> z"
+    thus "Sup A \<le> z"
+      apply (cases z)
+      apply (auto intro!: Sup_least simp add: Sup_top_def less_eq_top_def)
+      apply (metis top.simps(4))
+      by (metis (full_types) top.simps(5))
+  qed
+end
+
+lemma top_bind [simp]: "f \<hookleftarrow> top = top" by (simp add: top_top_def)
+
+end
