WeakTrioid/RelyGuarantee.thy
@@ -10,52 +10,6 @@ class rg_algebra = weak_trioid + meet_semilattice +
   and inv_par_closed: "\<lbrakk>r \<in> I; s \<in> I\<rbrakk> \<Longrightarrow> (r\<parallel>s) \<in> I"
   and inv_meet_closed: "\<lbrakk>r \<in> I; s \<in> I\<rbrakk> \<Longrightarrow> (r \<sqinter> s) \<in> I"
 
-locale rg_module =
-  fixes mod :: "'a::rg_algebra \<Rightarrow> 'b::boolean_algebra \<Rightarrow> 'b" (infixr "\<Colon>" 60)
-  assumes mod_mult: "x \<cdot> y \<Colon> p \<le> y \<Colon> x \<Colon> p"
-  and mod_isor: "p \<le> q \<Longrightarrow> x \<Colon> p \<le> x \<Colon> q"
-  and mod_isol: "x \<le> y \<Longrightarrow> x \<Colon> p \<le> y \<Colon> p"
-
-begin
-
-definition quintuple :: "'a \<Rightarrow> 'a \<Rightarrow> 'b \<Rightarrow> 'a \<Rightarrow> 'b \<Rightarrow> bool" ("_, _ \<turnstile> \<lbrace>_\<rbrace> _ \<lbrace>_\<rbrace>") where
-  "r, g \<turnstile> \<lbrace>p\<rbrace> c \<lbrace>q\<rbrace> \<longleftrightarrow> r \<parallel> c \<Colon> p \<le> q \<and> c \<le> g \<and> r \<in> I \<and> g \<in> I"
-
-lemma inv_dist: "r \<in> I \<Longrightarrow> r\<parallel>(x\<cdot>y) \<le> (r\<parallel>x)\<cdot>(r\<parallel>y)"
-  by (metis rg_algebra_class.inv_def)
-
-lemma sequential:
-  assumes "r, g1 \<turnstile> \<lbrace>p\<rbrace> c1 \<lbrace>q\<rbrace>" and "r, g2 \<turnstile> \<lbrace>q\<rbrace> c2 \<lbrace>s\<rbrace>"
-  shows "r, (g1 \<parallel> g2) \<turnstile> \<lbrace>p\<rbrace> c1 \<cdot> c2 \<lbrace>s\<rbrace>"
-proof -
-  have r_inv: "r \<in> I"
-    by (metis assms(1) quintuple_def)
-
-  {
-    have "r \<parallel> (c1 \<cdot> c2) \<Colon> p \<le> (r \<parallel> c1) \<cdot> (r \<parallel> c2) \<Colon> p"
-      by (metis inv_dist mod_isol r_inv)
-    also have "... \<le> r \<parallel> c2 \<Colon> r \<parallel> c1 \<Colon> p"
-      by (metis mod_mult)
-    also have "... \<le> r \<parallel> c2 \<Colon> q"
-      by (metis assms(1) mod_isor quintuple_def)
-    also have "... \<le> s"
-      by (metis assms(2) quintuple_def)
-    finally have "r \<parallel> (c1 \<cdot> c2) \<Colon> p \<le> s" .
-  }
-  moreover
-  {
-    have "c1 \<cdot> c2 \<le> g1 \<cdot> g2"
-      by (metis assms(1) assms(2) mult_isol_var quintuple_def)
-    also have "... \<le> g1 \<parallel> g2"
-      by (metis assms(1) assms(2) inv_mult_par quintuple_def)
-    finally have "c1 \<cdot> c2 \<le> g1 \<parallel> g2" .
-  }
-  ultimately show ?thesis
-    by (metis assms(1) assms(2) inv_par_closed quintuple_def)
-qed
-
-end
-
 begin
 
 definition guarantee_relation :: "'a \<Rightarrow> 'a \<Rightarrow> bool" ("_ guar _" [99, 99] 100) where
@@ -124,12 +78,12 @@ qed
 
 theorem sequential_composition:
   assumes "\<lbrace>a, r\<rbrace> b \<lbrace>c, g\<rbrace>" and "\<lbrace>c, r'\<rbrace> b' \<lbrace>c', g'\<rbrace>"
-  shows "\<lbrace>a, r \<sqinter> r'\<rbrace> b\<cdot>b' \<lbrace>c', g\<cdot>g'\<rbrace>"
+  shows "\<lbrace>a, r \<sqinter> r'\<rbrace> b\<cdot>b' \<lbrace>c', g\<parallel>g'\<rbrace>"
 proof -
   have "b\<cdot>b' \<le> g\<cdot>g'"
     by (metis assms(1) assms(2) guarantee_relation_def jones_quintuples_def mult_isol_var)
-  hence guarantee: "(b\<cdot>b') guar (g\<cdot>g')"
-    by (metis assms(1) assms(2) inv_mult_closed guarantee_relation_def jones_quintuples_def)
+  hence guarantee: "(b\<cdot>b') guar (g\<parallel>g')"
+    by (metis (full_types) assms(1) assms(2) guarantee_relation_def inv_mult_par inv_par_closed jones_quintuples_def order_trans)
   have "(r \<sqinter> r') \<in> I"
     by (metis assms(1) assms(2) jones_quintuples_def inv_meet_closed)
   hence "(r \<sqinter> r')\<parallel>(b\<cdot>b') \<le> ((r \<sqinter> r')\<parallel>b)\<cdot>((r \<sqinter> r')\<parallel>b')"
@@ -171,7 +125,7 @@ lemma guar_trancl: "b guar g \<Longrightarrow> b\<^sup>+ guar g"
   apply (simp only: guarantee_relation_def)
   apply (subgoal_tac "1 + g \<cdot> b \<le> g")
   apply (metis mult_onel trancl_inductr)
-  by (metis add_comm add_iso inv_def inv_idem_mult leq_def mult_isor)
+  by (metis add_commute add_iso inv_def inv_idem_mult leq_def mult_isor)
 
 theorem rg_transcl: "\<lbrace>a, r\<rbrace> b \<lbrace>a, g\<rbrace> \<Longrightarrow> \<lbrace>a, r\<rbrace> b\<^sup>+ \<lbrace>a, g\<rbrace>"
   by (metis guar_trancl inv_def iteration2 jones_quintuples_def)
@@ -181,5 +135,50 @@ theorem rg_star: "\<lbrakk>\<lbrace>a\<rbrace> r \<lbrace>a\<rbrace>; \<lbrace>a
 
 end
 
+locale rg_module =
+  fixes mod :: "'a::rg_algebra \<Rightarrow> 'b::boolean_algebra \<Rightarrow> 'b" (infixr "\<Colon>" 60)
+  assumes mod_mult: "x \<cdot> y \<Colon> p \<le> y \<Colon> x \<Colon> p"
+  and mod_isor: "p \<le> q \<Longrightarrow> x \<Colon> p \<le> x \<Colon> q"
+  and mod_isol: "x \<le> y \<Longrightarrow> x \<Colon> p \<le> y \<Colon> p"
+
+begin
+
+definition quintuple :: "'a \<Rightarrow> 'a \<Rightarrow> 'b \<Rightarrow> 'a \<Rightarrow> 'b \<Rightarrow> bool" ("_, _ \<turnstile> \<lbrace>_\<rbrace> _ \<lbrace>_\<rbrace>") where
+  "r, g \<turnstile> \<lbrace>p\<rbrace> c \<lbrace>q\<rbrace> \<longleftrightarrow> r \<parallel> c \<Colon> p \<le> q \<and> c \<le> g \<and> r \<in> I \<and> g \<in> I"
+
+lemma inv_dist: "r \<in> I \<Longrightarrow> r\<parallel>(x\<cdot>y) \<le> (r\<parallel>x)\<cdot>(r\<parallel>y)"
+  by (metis rg_algebra_class.inv_def)
+
+lemma sequential:
+  assumes "r, g1 \<turnstile> \<lbrace>p\<rbrace> c1 \<lbrace>q\<rbrace>" and "r, g2 \<turnstile> \<lbrace>q\<rbrace> c2 \<lbrace>s\<rbrace>"
+  shows "r, (g1 \<parallel> g2) \<turnstile> \<lbrace>p\<rbrace> c1 \<cdot> c2 \<lbrace>s\<rbrace>"
+proof -
+  have r_inv: "r \<in> I"
+    by (metis assms(1) quintuple_def)
+
+  {
+    have "r \<parallel> (c1 \<cdot> c2) \<Colon> p \<le> (r \<parallel> c1) \<cdot> (r \<parallel> c2) \<Colon> p"
+      by (metis inv_dist mod_isol r_inv)
+    also have "... \<le> r \<parallel> c2 \<Colon> r \<parallel> c1 \<Colon> p"
+      by (metis mod_mult)
+    also have "... \<le> r \<parallel> c2 \<Colon> q"
+      by (metis assms(1) mod_isor quintuple_def)
+    also have "... \<le> s"
+      by (metis assms(2) quintuple_def)
+    finally have "r \<parallel> (c1 \<cdot> c2) \<Colon> p \<le> s" .
+  }
+  moreover
+  {
+    have "c1 \<cdot> c2 \<le> g1 \<cdot> g2"
+      by (metis assms(1) assms(2) mult_isol_var quintuple_def)
+    also have "... \<le> g1 \<parallel> g2"
+      by (metis assms(1) assms(2) inv_mult_par quintuple_def)
+    finally have "c1 \<cdot> c2 \<le> g1 \<parallel> g2" .
+  }
+  ultimately show ?thesis
+    by (metis assms(1) assms(2) inv_par_closed quintuple_def)
+qed
+
+end
 
 end
